state equivalence

AAM.v
@@ -2,75 +2,90 @@
 
 Require Export SfLib.
 
+Inductive id : Type := 
+  Id : nat -> id.
+
+Definition beq_id X1 X2 :=
+  match (X1, X2) with
+    (Id n1, Id n2) => beq_nat n1 n2
+  end.
+
+Theorem beq_id_refl : forall X,
+  true = beq_id X X.
+Proof. destruct X. apply beq_nat_refl. Qed.
+
 (* ###################################################################### *)
 
 Inductive expr : Type :=
-  | var : id -> expr
-  | app : expr -> expr -> expr
-  | abs : id -> expr -> expr.
+  | e_var : id -> expr
+  | e_app : expr -> expr -> expr
+  | e_abs : id -> expr -> expr.
+
+Inductive val : Type :=
+  | v_abs : id -> expr -> val.
 
 Tactic Notation "expr_cases" tactic(first) ident(c) :=
   first;
-  [ Case_aux c "var" | Case_aux c "app" | Case_aux c "abs" ].
+  [ Case_aux c "e_var" | Case_aux c "e_app" | Case_aux c "e_abs" ].
 
 (* ###################################################################### *)
 
 Module CEK.
 
-Inductive val : Type :=
-  | clo : id -> expr -> partial_map val -> val.
+Inductive env : Type :=
+  | env_empty : env
+  | env_extend : env -> id -> (val * env) -> env.
 
-Definition env : Type := partial_map val.
+Fixpoint env_lookup p x :=
+  match p with
+    | env_empty => None
+    | env_extend q y (v, p') =>
+      if beq_id x y then Some (v, p') else env_lookup q x
+  end.
 
-Inductive frame : Type :=
-  | ar : expr -> frame
-  | fn : val -> frame.
-
-Definition kont : Type := list frame.
+Inductive kont : Type :=
+  | mt : kont
+  | ar : expr -> env -> kont -> kont
+  | fn : val -> env -> kont -> kont.
 
 Inductive state : Type :=
   | ev : expr -> env -> kont -> state
-  | ap : val -> kont -> state.
+  | ap : val -> env -> kont -> state.
 
 Definition inj : expr -> state :=
-  fun e => ev e empty [].
+  fun e => ev e env_empty mt.
 
 Reserved Notation "s1 '==>' s2" (at level 40).
 
 Inductive step : state -> state -> Prop :=
-  | cek1 :
-      forall x p k v,
-        p x = Some v ->
-        ev (var x) p k
-        ==>
-        ap v k
-  | cek2 :
+  | cek0 :
       forall x e p k,
-        ev (abs x e) p k
+        ev (e_abs x e) p k
         ==>
-        ap (clo x e p) k
+        ap (v_abs x e) p k
+  | cek1 :
+      forall x p k v p',
+        env_lookup p x = Some (v, p') ->
+        ev (e_var x) p k
+        ==>
+        ap v p' k
+  | cek2 :
+      forall e0 e1 p k,
+        ev (e_app e0 e1) p k
+        ==>
+        ev e0 p (ar e1 p k)
   | cek3 :
-      forall e1 e2 p k,
-        ev (app e1 e2) p k
+      forall v p e p' k,
+        ap v p (ar e p' k)
         ==>
-        ev e1 p (ar e2 :: k)
+        ev e p' (fn v p k)
   | cek4 :
-      forall x e p e2 k,
-        ap (clo x e p) (ar e2 :: k)
+      forall v p x e p' k,
+        ap v p (fn (v_abs x e) p' k)
         ==>
-        ev e2 p (fn (clo x e p) :: k)
-  | cek5 :
-      forall x e p v2 k,
-        ap v2 (fn (clo x e p) :: k)
-        ==>
-        ev e (extend p x v2) k
+        ev e (env_extend p' x (v, p)) k
 
 where "s1 '==>' s2" := (step s1 s2).
-
-Tactic Notation "step_cases" tactic(first) ident(c) :=
-  first;
-  [ Case_aux c "cek1" | Case_aux c "cek2" | Case_aux c "cek3"
-    | Case_aux c "cek4" | Case_aux c "cek5" ].
 
 Hint Constructors step.
 
@@ -78,17 +93,18 @@ Notation "s1 '==>*' s2" := (multi step s1 s2) (at level 40).
 
 Example ex1 :
   forall x y,
-    inj (app (abs x (var x)) (abs y (var y)))
+    inj (e_app (e_abs x (e_var x)) (e_abs y (e_var y)))
     ==>*
-    ap (clo y (var y) empty) [].
+    ap (v_abs y (e_var y)) env_empty mt.
 Proof.
   intros. unfold inj.
-  eapply multi_step. auto.
-  eapply multi_step. auto.
-  eapply multi_step. auto.
-  eapply multi_step. auto.
-  eapply multi_step. auto.
-  eapply multi_step. apply cek1. apply extend_eq.
+  eapply multi_step. apply cek2.
+  eapply multi_step. apply cek0.
+  eapply multi_step. apply cek3.
+  eapply multi_step. apply cek0.
+  eapply multi_step. apply cek4.
+  eapply multi_step. apply cek1.
+    simpl. rewrite <- beq_id_refl. reflexivity.
   apply multi_refl.
 Qed.
 
@@ -100,66 +116,74 @@ Module CESK.
 
 Definition addr : Type := id.
        
-Inductive val : Type :=
-  | clo : id -> expr -> partial_map addr -> val.
+Inductive env : Type :=
+  | env_empty : env
+  | env_extend : env -> id -> addr -> env.
 
-Definition env : Type := partial_map addr.
+Definition storable : Type := (val * env)%type.
 
-Definition storable : Type := val.
+Inductive store : Type :=
+  | store_empty : store
+  | store_extend : store -> addr -> storable -> store.
 
-Definition store : Type := partial_map storable.
+Fixpoint env_lookup p x :=
+  match p with
+    | env_empty => None
+    | env_extend q y a =>
+      if beq_id x y then Some a else env_lookup q x
+  end.
 
-Inductive frame : Type :=
-  | ar : expr -> frame
-  | fn : val -> frame.
+Fixpoint store_lookup s a :=
+  match s with
+    | store_empty => None
+    | store_extend t b (v, p') =>
+      if beq_id a b then Some (v, p') else store_lookup t a
+  end.
 
-Definition kont : Type := list frame.
+Inductive kont : Type :=
+  | mt : kont
+  | ar : expr -> env -> kont -> kont
+  | fn : val -> env -> kont -> kont.
 
 Inductive state : Type :=
-  | ev : expr -> env -> store -> kont -> state
-  | ap : val -> store -> kont -> state.
+  | ev : expr -> env -> store -> kont -> nat -> state
+  | ap : val -> env -> store -> kont -> nat -> state.
 
 Definition inj : expr -> state :=
-  fun e => ev e empty empty [].
+  fun e => ev e env_empty store_empty mt 0.
 
 Reserved Notation "s1 '==>' s2" (at level 40).
 
 Inductive step : state -> state -> Prop :=
+  | cesk0 :
+      forall x e p s k n,
+        ev (e_abs x e) p s k n
+        ==>
+        ap (v_abs x e) p s k n
   | cesk1 :
-      forall x p s k a v,
-        p x = Some a ->
-        s a = Some v ->
-        ev (var x) p s k
+      forall x p s k a v p' n,
+        env_lookup p x = Some a ->
+        store_lookup s a = Some (v, p') ->
+        ev (e_var x) p s k n
         ==>
-        ap v s k
+        ap v p' s k n
   | cesk2 :
-      forall x e p s k,
-        ev (abs x e) p s k
+      forall e0 e1 p s k n,
+        ev (e_app e0 e1) p s k n
         ==>
-        ap (clo x e p) s k
+        ev e0 p s (ar e1 p k) n
   | cesk3 :
-      forall e1 e2 p s k,
-        ev (app e1 e2) p s k
+      forall v p s e p' k n,
+        ap v p s (ar e p' k) n
         ==>
-        ev e1 p s (ar e2 :: k)
+        ev e p' s (fn v p k) n
   | cesk4 :
-      forall x e p s e2 k,
-        ap (clo x e p) s (ar e2 :: k)
+      forall v p s x e p' k n,
+        ap v p s (fn (v_abs x e) p' k) n
         ==>
-        ev e2 p s (fn (clo x e p) :: k)
-  | cesk5 :
-      forall x e p s v2 k a,
-        s a = None ->
-        ap v2 s (fn (clo x e p) :: k)
-        ==>
-        ev e (extend p x a) (extend s a v2) k
+        ev e (env_extend p' x (Id n)) (store_extend s (Id n) (v, p)) k (n + 1)
 
 where "s1 '==>' s2" := (step s1 s2).
-
-Tactic Notation "step_cases" tactic(first) ident(c) :=
-  first;
-  [ Case_aux c "cesk1" | Case_aux c "cesk2" | Case_aux c "cesk3"
-    | Case_aux c "cesk4" | Case_aux c "cesk5" ].
 
 Hint Constructors step.
 
@@ -167,19 +191,116 @@ Notation "s1 '==>*' s2" := (multi step s1 s2) (at level 40).
 
 Example ex1 :
   forall x y,
-    inj (app (abs x (var x)) (abs y (var y)))
+    inj (e_app (e_abs x (e_var x)) (e_abs y (e_var y)))
     ==>*
-    ap (clo y (var y) empty) (extend empty (Id 0) (clo y (var y) empty)) [].
+    ap (v_abs y (e_var y)) env_empty (store_extend store_empty (Id 0) (v_abs y (e_var y), env_empty)) mt 1.
 Proof.
   intros. unfold inj.
-  eapply multi_step. auto.
-  eapply multi_step. auto.
-  eapply multi_step. auto.
-  eapply multi_step. auto.
-  eapply multi_step. apply cesk5. auto.
-  eapply multi_step. apply cesk1 with (Id 0). apply extend_eq.
-    unfold extend. simpl. auto.
+  eapply multi_step. apply cesk2.
+  eapply multi_step. apply cesk0.
+  eapply multi_step. apply cesk3.
+  eapply multi_step. apply cesk0.
+  eapply multi_step. apply cesk4.
+  eapply multi_step. eapply cesk1.
+    simpl. rewrite <- beq_id_refl. reflexivity. reflexivity.
   apply multi_refl.
 Qed.
 
 End CESK.
+
+Tactic Notation "CEK.step_cases" tactic(first) ident(c) :=
+  first;
+  [ Case_aux c "cek0" | Case_aux c "cek1" | Case_aux c "cek2"
+    | Case_aux c "cek3" | Case_aux c "cek4" | Case_aux c "cek5" ].
+
+Tactic Notation "CESK.step_cases" tactic(first) ident(c) :=
+  first;
+  [ Case_aux c "cesk0" | Case_aux c "cesk1" | Case_aux c "cesk2"
+    | Case_aux c "cesk3" | Case_aux c "cesk4" | Case_aux c "cesk5" ].
+
+Fixpoint cesk_cek_env p s n :=
+  match p with
+    | CESK.env_empty => CEK.env_empty
+    | CESK.env_extend q x a =>
+      match n with
+        | 0 => CEK.env_empty (* error *)
+        | S n' =>
+          match CESK.store_lookup s a with
+            | None => CEK.env_empty (* error *)
+            | Some (v, p') =>
+              CEK.env_extend (cesk_cek_env q s n') x (v, (cesk_cek_env p' s n'))
+          end
+      end
+  end.
+
+Fixpoint cesk_cek_kont k s n :=
+  match k with
+    | CESK.mt => CEK.mt
+    | CESK.ar e p k' =>
+      CEK.ar e (cesk_cek_env p s n) (cesk_cek_kont k' s n)
+    | CESK.fn v p k' =>
+      CEK.fn v (cesk_cek_env p s n) (cesk_cek_kont k' s n)
+  end.
+
+Fixpoint cesk_cek_state st :=
+  match st with
+    | CESK.ev e p s k n =>
+      CEK.ev e (cesk_cek_env p s n) (cesk_cek_kont k s n)
+    | CESK.ap v p s k n =>
+      CEK.ap v (cesk_cek_env p s n) (cesk_cek_kont k s n)
+  end.
+
+Theorem cesk_cek_inj_eq :
+  forall e,
+    cesk_cek_state (CESK.inj e) = CEK.inj e.
+Proof. reflexivity. Qed.
+
+Inductive cek_cesk_env_sim : CEK.env -> CESK.env -> CESK.store -> Prop :=
+  | empty_sim :
+      forall s2,
+        cek_cesk_env_sim CEK.env_empty CESK.env_empty s2
+  | extend_sim :
+      forall q1 x1 v1 p1,
+        forall q2 x2 a2 v2 p2 s2,
+          x1 = x2 ->
+          v1 = v2 ->
+          cek_cesk_env_sim q1 q2 s2 ->
+          cek_cesk_env_sim p1 p2 s2 ->
+          CESK.store_lookup s2 a2 = Some (v2, p2) ->
+          cek_cesk_env_sim
+            (CEK.env_extend q1 x1 (v1, p1)) (CESK.env_extend q2 x2 a2) s2.
+
+Inductive cek_cesk_kont_sim : CEK.kont -> CESK.kont -> CESK.store -> Prop :=
+  | mt_sim :
+      forall s2,
+        cek_cesk_kont_sim CEK.mt CESK.mt s2
+  | ar_sim :
+      forall e1 p1 k1,
+        forall e2 p2 s2 k2,
+          e1 = e2 ->
+          cek_cesk_env_sim p1 p2 s2 ->
+          cek_cesk_kont_sim k1 k2 s2 ->
+          cek_cesk_kont_sim (CEK.ar e1 p1 k1) (CESK.ar e2 p2 k2) s2
+  | fn_sim :
+      forall v1 p1 k1,
+        forall v2 p2 s2 k2,
+          v1 = v2 ->
+          cek_cesk_env_sim p1 p2 s2 ->
+          cek_cesk_kont_sim k1 k2 s2 ->
+          cek_cesk_kont_sim (CEK.fn v1 p1 k1) (CESK.fn v2 p2 k2) s2.
+
+Inductive cek_cesk_state_sim : CEK.state -> CESK.state -> Prop :=
+  | ev_sim :
+      forall e1 p1 k1,
+        forall e2 p2 s2 k2 n2,
+          e1 = e2 ->
+          cek_cesk_env_sim p1 p2 s2 ->
+          cek_cesk_kont_sim k1 k2 s2 ->
+          cek_cesk_state_sim (CEK.ev e1 p1 k1) (CESK.ev e2 p2 s2 k2 n2)
+  | ap_sim :
+      forall v1 p1 k1,
+        forall v2 p2 s2 k2 n2,
+          v1 = v2 ->
+          cek_cesk_env_sim p1 p2 s2 ->
+          cek_cesk_kont_sim k1 k2 s2 ->
+          cek_cesk_state_sim (CEK.ap v1 p1 k1) (CESK.ap v2 p2 s2 k2 n2).
